Improve SimplSpill.

theories/Spilling/ExpVarsBounded.v
@@ -24,6 +24,7 @@ Inductive exp_vars_bounded : nat -> stmt -> Prop :=
 | BoundLet k x e s
   : cardinal (Exp.freeVars e) <= k
     -> exp_vars_bounded k s
+    -> k > 0
     -> exp_vars_bounded k (stmtLet x e s)
 | BoundReturn k e
   : cardinal (Op.freeVars e) <= k
@@ -51,7 +52,8 @@ Qed.
 
 Fixpoint exp_vars_bound (s:stmt) : nat :=
   match s with
-  | stmtLet x e s0 => max (cardinal (Exp.freeVars e)) (exp_vars_bound s0)
+  | stmtLet x e s0 =>
+    max (max (cardinal (Exp.freeVars e)) (exp_vars_bound s0)) 1
   | stmtIf e s1 s2 => max (cardinal (Op.freeVars e)) (max (exp_vars_bound s1) (exp_vars_bound s2))
   | stmtApp l Y => 0
   | stmtReturn e => cardinal (Op.freeVars e)
@@ -72,7 +74,8 @@ Lemma exp_vars_bound_sound s
 Proof.
   sind s; destruct s; simpl; econstructor;
     intros; inv_get; eauto using exp_vars_bounded_ge,Max.le_max_r,Max.le_max_l,list_max_get.
-  eapply exp_vars_bounded_ge; eauto.
-  rewrite <- list_max_get; eauto using get.
-  eapply Max.le_max_l.
+  - rewrite <- !Max.le_max_l. reflexivity.
+  - eapply exp_vars_bounded_ge; eauto.
+    rewrite <- list_max_get; eauto using get.
+    eapply Max.le_max_l.
 Qed.
